$$
A_x x + A_y  y = P_x \\
B_x  x + B_y  y = P_y \\
$$

solve for $y$ on first
$$
\begin{align}
	A_x  x + B_x  y &= P_x \\
	B_x  y &= -A_x  x + P_x \\
	y &= \frac{-A_x  x + P_x}{B_x}
\end{align}
$$
substitute $y$ in second
$$
\begin{align}
	A_y x + B_y y &= P_y \\
	A_y x + B_y \left( \frac{-A_x x + P_x}{B_x} \right) &= P_y
\end{align}
$$
solve for $x$
$$
\begin{align}
	A_y x + B_y \left( \frac{-A_x x + P_x}{B_x} \right) &= P_y \\
	A_y x + B_y \left( \frac{-A_x x}{B_x} + \frac{P_x}{B_x} \right) &= P_y \\
	A_y x + \left( \frac{-A_x B_y x}{B_x} + \frac{P_x B_y}{B_x} \right) &= P_y \\
	\frac{A_y B_x x}{B_x}  + \frac{-A_x B_y x}{B_x} + \frac{P_x B_y}{B_x}  &= P_y \\
	\frac{A_y B_x x  -A_x B_y x + P_x B_y}{B_x} &= P_y \\
	A_y B_x x -A_x B_y x + P_x B_y &= P_y B_x \\
	A_y B_x x -A_x B_y x &= P_y B_x - P_x B_y \\
	x(A_y B_x -A_x B_y) &= P_y B_x - P_x B_y \\
	x &= \frac{P_y B_x - P_x B_y}{A_y B_x -A_x B_y} \\
\end{align}
$$
final equations
$$
\begin{align}
	x &= \frac{P_y B_x - P_x B_y}{A_y B_x -A_x B_y} \\
	y &= \frac{-A_x  x + P_x}{B_x}
\end{align}
$$


